refactor/Proof/Application.v
@@ -57,7 +57,7 @@ Inductive papp : term -> term -> term -> Prop :=
 
 Hint Constructors papp : core.
 
-Notation "v ◐ vl ~-> e" := (papp v vl e) (at level 69).
+Notation "v · vl ⟹ e" := (papp v vl e) (at level 69).
 
 (** * Determinism *)
 
@@ -85,7 +85,7 @@ Proof.
                   end.  
   introv Val Vall P1 P2 Typ. gen e2 A.
   induction P1; intros.
-  - Case "Lit Topike".
+  - Case "Lit Toplike".
     dependent destruction P2; eauto.
   - Case "Lam Toplike".
     dependent destruction P2; eauto.
@@ -168,8 +168,314 @@ Qed.
 
 End papp_consistent.
 
+(** * Weakening Lemma *)
+
+Lemma typing_weakening_gen :
+  forall G E F e A,
+    typing (E ++ G) e A ->
+    uniq (E ++ F ++ G) ->
+    typing (E ++ F ++ G) e A.
+Proof.
+  introv Htyp.
+  gen F.
+  dependent induction Htyp; introv Henv; eauto.
+  pick fresh x and apply Ty_Lam.
+  rewrite_env (([(x,A)] ++ E) ++ F ++ G).
+  apply H0; eauto.
+  solve_uniq. assumption.
+Qed.
+
+Lemma typing_weakening :
+  forall E F e A,
+    typing E e A ->
+    uniq (F ++ E) ->
+    typing (F ++ E) e A.
+Proof.
+  intros.
+  rewrite_env (nil ++ F ++ E).
+  eapply typing_weakening_gen; eauto.
+Qed.
+
 (** * Subsitution Lemma *)
+
+Lemma typing_uniq :
+  forall E e T,
+    typing E e T -> uniq E.
+Proof.
+  introv Typ.
+  induction Typ; eauto.
+  - pick fresh x.
+    assert (J: uniq ((one (x,A)) ++ T)); eauto.
+    dependent destruction J; eauto.
+Qed.
+
+Lemma typing_subst_var_case :
+  forall E F u S T (z x : atom),
+    binds x T (F ++ [(z, S)] ++ E) ->
+    uniq (F ++ [(z, S)] ++ E) ->
+    typing E u S ->
+    typing (F ++ E) (substitution z u x) T.
+Proof.
+  introv H J K.
+  simpl.
+  destruct (x == z).
+  - subst. assert (T = S).
+    eapply binds_mid_eq; eauto. subst.
+    eapply typing_weakening; eauto.
+  - eapply Ty_Var; eauto.
+Qed.
+
+Lemma fv_open_lower :
+  forall e1 e2 k,
+    fv e1 [<=] fv (open_rec k e2 e1).
+Proof with auto.
+  intros.
+  generalize dependent k.
+  induction e1; intros; simpl; try fsetdec...
+  - specialize (IHe1_1 k).
+    specialize (IHe1_2 k).
+    fsetdec...
+  - specialize (IHe1_1 k).
+    specialize (IHe1_2 k).
+    fsetdec...
+Qed.
+
+Lemma fv_in_dom :
+  forall T e A,
+    typing T e A -> fv e [<=] dom T.
+Proof.
+  introv Htyp.
+  dependent induction Htyp; simpl; try fsetdec; eauto.
+  - apply binds_In in H0.
+    fsetdec.
+  - pick fresh x. 
+    assert ((fv (open e x)) [<=] (dom ((one (x, A)) ++ T))) by eauto.
+    simpl in *.
+    assert (fv e [<=] fv (open e x)).
+    eapply fv_open_lower.
+    assert (fv e [<=] add x (dom T)).
+    fsetdec.
+    eapply add_notin_context; eauto.
+Qed.    
+
+Lemma subst_value :
+  forall e z u A ,
+    typing nil e A -> substitution z u e = e.
+Proof with auto.
+  intros.
+  apply fv_in_dom in H...
+  simpl in H...
+  eapply subst_fresh; eauto.
+  fsetdec.
+Qed.
+
+Lemma typing_subst:
+  forall E F e u S T (z : atom),
+    typing (F ++ (one (z, S)) ++ E) e T ->
+    typing E u S ->
+    typing (F ++ E) (substitution z u e) T.
+Proof.
+  introv He Hu.
+  remember (F ++ (one (z, S)) ++ E) as E'.
+  gen F.
+  induction He; intros.
+  - subst. eapply Ty_Int; eauto.
+  - subst. eapply typing_subst_var_case; eauto.
+  - subst. simpl.
+    pick fresh y and apply Ty_Lam; eauto.
+    rewrite subst_open_var; eauto.
+    rewrite_env (([(y, A)] ++ F) ++ E).
+    eapply H0; eauto.
+    Unshelve. eauto.
+  - subst. simpl.
+    eapply Ty_Ann; eauto.
+  - subst. simpl.
+    eapply Ty_App; eauto.
+  - subst. simpl.
+    eapply Ty_Mrg; eauto.
+  - subst. simpl.
+    pose proof (subst_value u1 z u _ He1) as St1.
+    pose proof (subst_value u2 z u _ He2) as St2.
+    rewrite St1. rewrite St2.
+    eapply Ty_Mrg_Uv; eauto.
+Qed.
+
+Lemma typing_rename : forall (x y : atom) E e T1 T2,
+  x `notin` fv e -> y `notin` (dom E `union` fv e) ->
+  typing ((one (x, T1)) ++ E) (open e x) T2 ->
+  typing ((one (y, T1)) ++ E) (open e y) T2.
+Proof.
+  introv Fr1 Fr2 Htyp.
+  destruct (x == y).
+  - subst. eauto.
+  - assert (J : uniq ((one (x, T1)) ++ E)).
+    eapply typing_uniq; eauto.
+    assert (J': uniq E).
+    inversion J; eauto.
+    rewrite (@subst_intro x); eauto.
+    rewrite_env (nil ++ (one (y, T1)) ++ E).
+    eapply typing_subst with (S := T1).
+    simpl_env.
+    eapply typing_weakening_gen; eauto.
+    eapply Ty_Var; eauto.
+Qed.
+
+(** substitution lemma, 
+stating that substituting a (closed, well-typed) term s for a variable x in a term t preserves the type of t *)
+
+Lemma substitution_lemma :
+   forall F E x v e A B C,
+    typing (F ++ [(x, A)] ++ E) e B ->
+    typing nil v C ->
+    isosub C A ->
+    (exists D, typing (F ++ E) (substitution x v e) D /\ isosub D B).
+Proof.
+  introv Typ Typv Isub. remember (F ++ [(x, A)] ++ E) as E'. gen F.
+  induction Typ; intros; simpl; subst; eauto.
+  - Case "Var".
+    destruct (x0 == x); eauto. subst.
+    eapply binds_mid_eq in H0; eauto. subst.
+    exists C. split; eauto.
+    eapply typing_weakening; eauto.
+    rewrite_env (E ++ nil).
+    eapply typing_weakening; eauto.
+    solve_uniq.
+  - Case "Lam".
+    (* TODO: automation *)
+    exists (Arr A0 B). split; eauto.
+    pick fresh y.
+    assert (y `notin` L) by eauto.
+    assert ((([(y, A0)] ++ (F ++ ([(x, A)] ++ E))) = (([(y, A0)] ++ F) ++ ([(x, A)] ++ E)))).
+    rewrite_env (([(y, A0)] ++ F) ++ ([(x, A)] ++ E)). auto.
+    pose proof (H0 y H2 ([(y, A0)] ++ F) H3).
+    destruct H4. destruct H4.
+    eapply (Ty_Lam (union L
+                  (union (singleton x)
+                     (union (dom E)
+                        (union (dom F)
+                           (union (singleton x) (union (fv v) (fv e)))))))  (F ++ E) A0 B x0); eauto.
+    intros.
+    assert ((substitution x v (open e y)) = (open (substitution x v e) y)).
+    symmetry.
+    eapply subst_open_var; eauto.
+    rewrite H7 in H4.    
+    rewrite_env ([(y, A0)] ++ (F ++ E)) in H4.
+    eapply (typing_rename y x1); eauto 3.
+    eapply subst_notin_fv; eauto.
+    eapply notin_union; eauto.
+    eapply subst_notin_fv; eauto.
+    eapply isosub_to_sub1 in H5.
+    eapply sub_transitivity; eauto.
+    Unshelve. eauto.
+  - Case "Ann".
+    exists A0. split; eauto.
+    pose proof (IHTyp F) as IH. destruct IH; eauto. destruct_conjs.
+    eapply Ty_Ann; eauto. eapply isosub_to_sub1 in H1.
+    eapply sub_transitivity; eauto.
+  - Case "App".
+    pose proof (IHTyp1 F) as IH1. pose proof (IHTyp2 F) as IH2.
+    destruct IH1; destruct IH2; eauto. destruct_conjs.
+    eapply appsub_iso in H; eauto. destruct H. destruct H.
+    exists x2. split; eauto.
+  - Case "Merge".
+    pose proof (IHTyp1 F) as IH1. pose proof (IHTyp2 F) as IH2.
+    destruct IH1; destruct IH2; eauto. destruct_conjs.
+    exists (And x0 x1). split; eauto.
+    eapply Ty_Mrg; eauto. eapply disjoint_iso_l; eauto.
+  - Case "Merge V".
+    exists (And A0 B). split; eauto.
+    pose proof (subst_value u1 x v _ Typ1) as Rw1.
+    pose proof (subst_value u2 x v _ Typ2) as Rw2.
+    rewrite Rw1. rewrite Rw2.
+    eapply Ty_Mrg_Uv; eauto.
+Qed.
 
 (** * Preservation *)
 
+Section papp_preservation.
+
+Lemma papp_uvalue :
+  forall v vl e A B,
+    value v -> value vl ->
+    typing nil v A -> typing nil vl B ->
+    papp v vl e ->
+    uvalue e.
+Proof.
+  introv Val Vall Typ Typl Pa. gen A B.
+  induction Pa; intros; eauto 5;
+    try solve [dependent destruction Val; dependent destruction Typ; eauto].
+Qed.  
+
+Lemma papp_preservation :
+  forall v vl e A B C,
+    value v -> value vl ->
+    typing nil v A ->
+    typing nil vl B ->
+    appsub (Some B) A C ->
+    papp v vl e ->
+    (exists D, typing nil e D /\ isosub D C).
+Proof.
+  Ltac solver1 := repeat match goal with
+                         | [Typ: typing nil ?v ?A, Val: value ?v, Pt: ptype ?v _ |- _] =>
+                             (pose proof (typing_to_ptype _ _ (value_is_uvalue _ Val) Typ); subst_ptype; clear Pt)
+                         end.
+  introv Val Vall Typ Typl As Pa. gen A B C.
+  induction Pa; intros.
+  - Case "Lit Toplike".
+    dependent destruction Typ. exists B. split.
+    + eapply Ty_Ann; eauto. eapply sub_toplike_super; eauto.
+    + dependent destruction As; eauto.
+  - Case "Lam Toplike".
+    dependent destruction Typ. exists D. split.
+    + eapply Ty_Ann; eauto. eapply sub_toplike_super; eauto.
+    + dependent destruction As; eauto.
+  - Case "Lam".    
+    repeat dependent destruction Typ. dependent destruction As.
+    dependent destruction Val.
+    match goal with
+    | [H: sub (Arr _ _) (Arr _ _) |- _] => (dependent destruction H; eauto)
+    end.
+    exists D. split; eauto.
+    match goal with
+    | [H: casting _ _ _ |- _] => (eapply casting_preservation in H; eauto; destruct H; destruct H)
+    end.
+    pick fresh y. rewrite (subst_intro y); eauto.
+    assert (Fr': y `notin` L) by eauto.
+    pose proof (H4 y Fr').
+    rewrite_env (nil ++ [(y, A)] ++ nil) in H9.
+    pose proof (substitution_lemma nil nil y vl' (open e y) A C0 x) as Sl.
+    destruct Sl as [x' Sl']; eauto. destruct Sl'.
+    eapply Ty_Ann; eauto.
+    eapply isosub_to_sub1 in H11; eauto.
+    eapply sub_transitivity; eauto 3. eapply sub_transitivity; eauto.
+  - Case "Merge L".
+    dependent destruction Val. dependent destruction Typ;
+      dependent destruction As; eauto 3; solver1; eauto.
+  - Case "Merge R".
+    dependent destruction Val. dependent destruction Typ;
+      dependent destruction As; eauto 3; solver1; eauto.
+  - Case "Merge P".
+    dependent destruction Val. dependent destruction Typ.
+    + solver1.
+      dependent destruction As; eauto.
+      pose proof (IHPa1 Val1 Vall _ Typ1 _ Typl _ As1).
+      pose proof (IHPa2 Val2 Vall _ Typ2 _ Typl _ As2).
+      destruct_conjs. exists (And H H0). split; eauto.
+      eapply Ty_Mrg; eauto.
+      assert (disjoint D1 D2). eapply disjoint_appsub; eauto.
+      eapply disjoint_iso_l; eauto.
+    + solver1.
+      dependent destruction As; eauto.
+      pose proof (IHPa1 Val1 Vall _ Typ1 _ Typl _ As1).
+      pose proof (IHPa2 Val2 Vall _ Typ2 _ Typl _ As2).
+      destruct_conjs. exists (And H H0). split; eauto.
+      pose proof (papp_uvalue _ _ _ _ _ Val1 Vall Typ1 Typl Pa1).
+      pose proof (papp_uvalue _ _ _ _ _ Val2 Vall Typ2 Typl Pa2).
+      eapply Ty_Mrg_Uv; eauto 3.
+      pose proof (papp_consistent v1 v2 vl e1 e2 A0 B0 B1) as Pc.
+      eapply Pc; eauto.    
+Qed.
+
+End papp_preservation.
+    
 (** * Progress *)
